%! TEX root = ./main.tex

\section{Functional Dependency}
\begin{itemize}
    \ides{Redundancy}
        \begin{itemize}
            \item Keep same data in multiple relations and/or multiple tuples
            \icon Waste of storage space
            \icon Additional work to keep consistent
                \begin{itemize}
                    \item Else we get anomalies
                \end{itemize}
            \icon Hard to keep consistent
            \icon Additional code to keep consistent
            \ipro Improve locality
            \ipro Better performance
            \ipro Fault tolerance
            \ipro Availability
        \end{itemize}
    \item FD is one way to model and understand redundancy
    \item Models and helps to reason about redundant data
    \ides{FD Definition}
        \begin{itemize}
            \item For:
                \begin{itemize}
                    \ides{Relation Schema:} $R(A:D_A, B:D_B, C:D_C, D:D_D)$
                    \ides{Instance:} $R \subseteq D_A \times D_B \times D_C \times D_D$
                \end{itemize}
            \item Let $\alpha \subseteq R, \beta \subseteq R$
                \begin{itemize}
                    \item Subset of columns
                \end{itemize}
                \ides{Functional Dependency $\mathbf{\alpha \to \beta}$:} iff $\forall r, s \in R.\ r.\alpha = s.\alpha \implies r.\beta = s.\beta$
                    \begin{itemize}
                        \item I.e. $\alpha \to \beta \iff$ for any two tuples $r$ and $s$ in DB instance $R$, if $r$ and $s$ share the same values on columns $\alpha$, then they share the same values on column $\beta$
                        \item I.e. there is a mapping, mapping values in columns $\alpha$ to values in columns in $\beta$
                        \ides{Notation:} $R \models \alpha \to \beta$ if $R$ satisfies $\alpha \to \beta$
                    \end{itemize}
        \end{itemize}
        \ides{FD $\mathbf{\alpha \to \beta}$ is \textbf{minimal}:} iff $\forall A \in \alpha.\ (\alpha \setminus \{A\}) \not \to \beta$
            \begin{itemize}
                \ides{Notation:} $\alpha \to \overset{.}{} \beta$
            \end{itemize}
    \ides{Keys}
        \begin{itemize}
            \ides{Superkey} is $\alpha \subseteq \mc{R} \iff \alpha \to \mc{R}$
                \begin{itemize}
                    \item I.e. if we know the value of columns $\alpha$ we know all values of all columns
                    \item All columns together are a trivial candidate key
                \end{itemize}
            \ides{Candidate Key} is $\alpha \subseteq \mc{R} \iff \alpha \to \overset{.}{} \mc{R}$
                \begin{itemize}
                    \item I.e. a minimal super key
                \end{itemize}
        \end{itemize}
    \ides{Implication/Inference}
        \begin{itemize}
            \item Given:
                \begin{itemize}
                    \item Set $F$ of some FDs on schema $\mc{R}$
                    \item FD $\alpha \to \beta$ which is $\not\in F$
                \end{itemize}
            \item $F$ \textbf{implies} $\alpha \to \beta$ if every relation instance $R$ of $\mc{R}$ that satisfies all FDs on $F$ also satisfies $\alpha \to \beta$
            \ides{Notation:} $F \models \alpha \to \beta$
        \end{itemize}
    \ides{Derivation}
        \begin{itemize}
            \item Given:
                \begin{itemize}
                    \item Set $F$ of some FDs on schema $\mc{R}$
                    \item FD $\alpha \to \beta$ which is $\not\in F$
                \end{itemize}
            \item $F$ \textbf{derives} $\alpha \to \beta$ if there is a derivation (using Armstrong's axioms) from $F$ to $\alpha \to \beta$
            \ides{Notation:} $F \vdash \alpha \to \beta$
        \end{itemize}
    \ides{Closure}
        \begin{itemize}
            \item Given:
                \begin{itemize}
                    \item Set $F$ of some FDs on schema $\mc{R}$
                    \item Set of attributes $\alpha \subseteq \mc{R}$
                \end{itemize}
            \item \textbf{Closure} of $\alpha$ is the set of all attributes $y \in \mc{R}$, such that $\alpha \to y$ can be derived from $F$
            \ides{Notation:} $\alpha^+$
            \item $\alpha^+ = \{y \in \mc{R} \mid F \vdash \alpha \to y\}$
            \item $F \vdash \alpha \to \beta \iff \beta \subseteq \alpha^+$
            \ides{Recipe:} Find $\alpha^+$
                \begin{itemize}
                    \item[1)] Set $\alpha^+$ to $\alpha$
                    \item[2)] For all $\beta \in \alpha$ check if there is a $\beta \to \gamma$ and add $\gamma$ to $\alpha^+$ if so
                    \item[3)] Repeat step 2 until $\alpha^+$ converges
                \end{itemize}
        \end{itemize}
    \ides{Minimal Basis/Cover}
        \begin{itemize}
            \ides{Goal:} Remove redundant FDs in a set of FDs
                \begin{itemize}
                    \item I.e. FDs which we can derive from the other FDs
                \end{itemize}
            \item Given: Set $F$ of some FDs
            \item A \textbf{Minimal Cover} of $F$ is a set $G \subseteq F$ with:
                \begin{itemize}
                    \item $G \equiv F$
                    \item All FDs in $G$ have the form $X \to \alpha$, where $\alpha$ is a single attribute
                    \item It is not possible to make $G$ smaller by:
                        \begin{itemize}
                            \item $G \setminus \{X \to \alpha\} \not\equiv G, \ \forall X \to \alpha \in G$
                                \begin{itemize}
                                    \item I.e. remove a FD
                                \end{itemize}
                            \item $(G \setminus \{X\alpha \to \beta\}) \cup \{X \to \beta\} \not\equiv G\ \forall X\alpha \to \beta \in G$
                                \begin{itemize}
                                    \item I.e. Remove an attribute from a FD
                                \end{itemize}
                        \end{itemize}
                \end{itemize}
            \ides{Recipe:} Compute minimal basis
                \begin{itemize}
                    \item[1)] Set $G$ to the set of FDs obtained from $F$ when decomposing the RHS of each FD to a single attribute
                    \item[2)] Remove trivial FDs
                        \begin{itemize}
                            \item I.e. all $a \to b$ where $b \subseteq a$
                        \end{itemize}
                    \item[3)] Remove all redundant attributes from the LHS of all FDs
                        \begin{itemize}
                            \item I.e. if $a \to b$ and $\exists x \in a$ such that $(a \setminus x) \to b$, replace $a \to b$ with $(a \setminus x) \to b$
                        \end{itemize}
                    \item[4)] Remove all redundant FDs
                        \begin{itemize}
                            \item I.e. if $a \to b$ and $\{b\} \subseteq \text{Closure}(F \setminus \{a \to b\}, a)$, remove $a \to b$ from $F$
                        \end{itemize}
                \end{itemize}
        \end{itemize}
    \ides{Equivalence}
        \begin{itemize}
            \item Given: Set $F$ and $G$ of FDs on schema $\mc{R}$
            \item $F$ and $G$ are \textbf{equivalent} if $F \models G$ and $G \models F$
            \ides{Notation:} $F \equiv G$
    \item Cardinalities define FD
    \item FD determine keys
        \end{itemize}
    \ides{Armstrong Axioms}
        \begin{itemize}
            \item Axioms:
                \begin{itemize}
                    \ides{Reflexivity:} $\alpha \subseteq \beta \implies \beta \to \alpha$
                        \begin{itemize}
                            \item Special case is $\mc{R} \to \alpha$
                            \item Trivial FDs
                        \end{itemize}
                    \ides{Augmentation:} $\alpha \to \beta \implies \alpha \gamma \to \beta \gamma$
                        \begin{itemize}
                            \item Where $\alpha \gamma := \alpha \cup \gamma$
                        \end{itemize}
                    \ides{Transitivity:} $\alpha \to \beta \wedge \beta \to \gamma \implies \alpha \to \gamma$
                \end{itemize}
            \item These axioms are both:
                \begin{itemize}
                    \ides{Sound:} $F \vdash \alpha \to \beta \implies F \models \alpha \to \beta$
                    \ides{Complete:} $F \models \alpha \to \beta \implies F \vdash \alpha \to \beta$
                \end{itemize}
            \item All other FDs can be implied from these axioms
        \end{itemize}
    \ides{Other Rules}
        \begin{itemize}
            \ides{Union:} $\alpha \to \beta \wedge \alpha \to \gamma \implies \alpha \to \beta \gamma$
            \ides{Composition:} $\alpha \to \beta \gamma \implies \alpha \to \beta \wedge \alpha \to \gamma$
            \ides{Pseudo Transitivity:} $\alpha \to \beta \wedge \beta \gamma \to \theta \implies \alpha \gamma \to \theta$
        \end{itemize}
    \ides{Composition of Relations}
        \begin{itemize}
            \ides{Goal:} Split bad relations into ones containing only one concept
                \begin{itemize}
                    \ides{Bad Relation:} Relation which combine several concepts
                \end{itemize}
            \ides{Lossless Decomposition} Of $R$ into $R_1, \dots, R_n$ if $R = R_1 \bowtie R_2 \bowtie \dots \bowtie R_n$
                \begin{itemize}
                    \item For $\mc{R} = \mc{R}_1 \cup \mc{R}_2$, decomposition $R_1 = \Pi_{\mc{R}_1}(R), R_2 = \Pi_{\mc{R}_2}(R)$ is lossless, if $(\mc{R}_1 \cap \mc{R}_2) \to \mc{R}_1 \vee (\mc{R}_1 \cap \mc{R}_2) \to \mc{R}_2$
                \end{itemize}
            \ides{Recipe:} Show given decomposition $R_1, R_2$ is lossy
                \begin{itemize}
                    \item Decomposition is lossless iff $R = R_1 \bowtie R_2$
                    \item Find some instance of the relations which serves as a counterexample
                \end{itemize}
            \ides{Recipe:} Show given decomposition $R_1, R_2$ is lossless
                \begin{itemize}
                    \item Decomposition is lossless if $(R_1 \cap R_2) \to R_i, i \in \{1, 2\}$
                \end{itemize}
            \ides{Preservation of Dependencies:} $\text{FD}(R)^+ = [\text{FD}(R_1) \cup \dots \cup \text{FD}(R_n)]^+$
        \end{itemize}
\end{itemize}
